SSA.v
@@ -12,7 +12,7 @@ Require Import LLIR.Block.
 
 Import ListNotations.
 
-Section VALIDITY.
+Section FUNC_VALIDITY.
   Variable f: func.
 
   Definition uses_have_defs :=
@@ -28,18 +28,30 @@ Section VALIDITY.
       DefinedAt f def' r ->
       def' = def.
 
+  Definition inst_does_not_use_defs :=
+    forall (def: node) (r: reg),
+      InstDefinedAt f def r -> ~InstUsedAt f def r.
+
   Definition blocks_are_valid :=
     forall (e: node),
       (exists (h: node), BasicBlock f h e) \/ (f.(fn_insts) ! e = None).
 
-  Record is_valid : Prop :=
+  Definition phi_or_inst :=
+    forall (def: node) (r: reg),
+      (InstDefinedAt f def r -> ~PhiDefinedAt f def r)
+      /\
+      (PhiDefinedAt f def r -> ~InstDefinedAt f def r).
+
+  Record valid_func : Prop :=
     { fn_uses_have_defs: uses_have_defs
     ; fn_defs_are_unique: defs_are_unique
     ; fn_blocks_are_valid: blocks_are_valid
+    ; fn_inst_does_not_use_defs: inst_does_not_use_defs
+    ; fn_phi_or_inst: phi_or_inst
     }.
 
   Theorem defs_dominate_uses:
-    is_valid ->
+    valid_func ->
     forall (def: node) (use: node) (r: reg),
       DefinedAt f def r ->
       UsedAt f use r ->
@@ -56,4 +68,36 @@ Section VALIDITY.
     generalize (Hdefs_are_unique def dom r Hdef Hdef').
     intros Heq. subst. auto.
   Qed.
-End VALIDITY.
+
+  Theorem inst_does_not_defs_uses:
+    valid_func ->
+    forall (def: node) (r: reg),
+      InstUsedAt f def r -> ~InstDefinedAt f def r.
+  Proof.
+    intros Hvalid def r Hused_at Hdefined_at.
+    destruct Hvalid as [_ _ _ Hno_use].
+    generalize (Hno_use def r Hdefined_at); intros contra.
+    contradiction.
+  Qed.
+
+  Theorem inst_def_single_reg:
+    forall (def: node) (r: reg) (r': reg),
+      InstDefinedAt f def r ->
+      InstDefinedAt f def r' ->
+      r = r'.
+  Proof.
+    intros def r r' Hdef Hdef'.
+    inversion Hdef; inversion Hdef'.
+    rewrite <- INST0 in INST; inversion INST; subst i0.
+    inversion DEFS; inversion DEFS0; subst; inversion H5; reflexivity.
+  Qed.
+End FUNC_VALIDITY.
+
+Section PROG_VALIDITY.
+  Variable p: prog.
+
+  Definition valid_prog (p: prog) :=
+    forall (n: name) (f: func),
+      Some f = p ! n -> valid_func f.
+
+End PROG_VALIDITY.
