Liveness.v
@@ -1,0 +1,17 @@
+(* This file is part of the LLIR Semantics project. *)
+(* Licensing information is available in the LICENSE file. *)
+(* (C) 2020 Nandor Licker. All rights reserved. *)
+
+Require Import Coq.Lists.List.
+Require Import LLIR.LLIR.
+Require Import LLIR.Dom.
+
+
+Inductive LiveAt: func -> reg -> node -> Prop :=
+  | live_at:
+    forall
+      (f: func) (r: reg) (n: node) (use: node) (p: list node)
+      (PATH: Path f n p use)
+      (NO_DEF: forall (def: node), In def p -> ~DefinedAt f def r)
+      (USE: UsedAt f use r),
+      LiveAt f r n.
