Signal.v
@@ -1,0 +1,10 @@
+(* This file is part of the LLIR Semantics project. *)
+(* Licensing information is available in the LICENSE file. *)
+(* (C) 2020 Nandor Licker. All rights reserved. *)
+
+
+Inductive signal :=
+  | SIGSEGV
+  | SIGBUS
+  | SIGFPE
+  .
